

---

# ASSSIGNMENT 2

---

PHYSICS 451

DATE FEBRUARY 25, 2026

JAYNARD KIGAS (30173694)

*The University of Calgary*



UNIVERSITY OF  
CALGARY

# Contents

Question 1	1
Question 1.a	1
Question 1.b	1
Question 2	2
Question 2.a	2
Question 2.b	2
Question 2.c	3
Question 2.d	4
Question 3	4
Question 3.a	4
Question 3.b	5
Question 3.c	6

## Question 1

Scaling Behavior (4 Points)

### Question 1.a

Near critical points, the self-similarity under rescaling leads to characteristic power-law singularities. These dependences may be disguised, however, by less-singular corrections to scaling. An experiment measures the susceptibility  $\chi(T)$  in a magnet for temperatures  $T$  slightly above the ferromagnetic transition temperature  $T_c$ . They find their data is fit well by the form

$$\chi(T) = A(T - T_c)^{-1.25} + B + C(T - T_c) + D(T - T_c)^{1.77} \quad (1.1)$$

Assuming this is the correct dependence near  $T_c$ , what is the critical exponent  $\gamma$

The critical exponent is the one belonging to the term that has the leading behavior. We can see that for the  $D$  term, a temperature around the critical temperature is still a small number. This is true with  $B$  and  $C$  as well since their exponent is 1. However, the exponent for  $A$  is negative. This means that when  $T \rightarrow T_c$ , we get a diverging term. This means that:

$$\gamma = -1.25 \quad (1.2)$$

### Question 1.b

The pair correlation function  $C(r, T) = \langle \sigma_i \sigma_{i+r} \rangle$  is measured in another, three-dimensional system just above  $T_c$ . It is found to be spherically symmetric, and of the form

$$C(r, T) = r^{-1.026} G(r(T - T_c)^{0.59}) \quad (1.3)$$

Where the function  $G(x)$  is found to be roughly  $\exp(-x)$ . What is the critical exponent  $\nu$ ?

The critical exponent comes from the how the correlation length diverges with  $(T - T_c)^{-\nu}$ . Since 0.59 is the exponent on this factor in our correlation function, we have:

$$\nu = 0.59 \quad (1.4)$$

## Question 2

The recursion relations for nonzero magnetic field

### Question 2.a

For nonzero magnetic field show that the function  $A(K, h)$  satisfies the relation:

$$2e^{h(s_1+s_3)/2} \cosh[K(s_1 + s_3) + h] = A(K, h)e^{K's_1s_3+h'(s_1+s_3)/2} \quad (2.1)$$

Let's do this by considering the combinations of spin states  $s_1$  and  $s_3$ . Let's start with  $s_1 = s_3 = +1$ .

$$2e^{h2/2} \cosh[2K + h] = A(K, h)e^{1K'+h'2/2} \quad (2.2)$$

This is then

$$A(K, h)e^{K'+h'} = 2e^h \cosh[2K + h] = e^{2K+2h} + e^{-2K} \quad (2.3)$$

Now let's go to the case where  $s_1 = s_3 = -1$

$$2e^{-h} \cosh[-2K + h] = A(K, h)e^{K'-h'} \quad (2.4)$$

$$A(K, h)e^{K'-h'} = e^{-2K} + e^{2K-2h} \quad (2.5)$$

Now for the case where the states are not equal

$$2e^0 \cosh[h] = A(K, h)e^{-K'+0} \quad (2.6)$$

$$A(K, h)e^{-K'} = e^h + e^{-h} \quad (2.7)$$

Wow these are all the relations we find in question 3.

### Question 2.b

Show that the recursion relations for nonzero magnetic field are

$$K' = \frac{1}{4} \ln \frac{\cosh(2K + h) \cosh(2K - h)}{\cosh^2 h} \quad (2.8)$$

$$h' = h + \frac{1}{2} \ln \left[ \frac{\cosh(2K + h)}{\cosh(2K - h)} \right] \quad (2.9)$$

and

$$\ln A(K, h) = \frac{1}{4} \ln [16 \cosh(2K + h) \cosh(2K - h) \cosh^2 h] \quad (2.10)$$

Let's start by multiplying equation 2.3 and 2.5, then divide by the square of 2.7.

$$e^{4K'} = \frac{(e^{2K+2h} + e^{-2K})(e^{-2K} + e^{2K-2h})}{(e^h + e^{-h})^2} \quad (2.11)$$

The product on the top:

$$(e^{2K+2h} + e^{-2K})(e^{-2K} + e^{2K-2h}) = (2e^h \cosh[2K+h])(2e^{-h} \cosh[-2K+h]) = 4 \cosh[2K+h] \cosh[-2K+h] \quad (2.12)$$

We then get:

$$e^{4K'} = \frac{4 \cosh[2K + h] \cosh[-2K + h]}{4 \cosh^2[h]} \quad (2.13)$$

$$K' = \frac{1}{4} \ln \frac{\cosh[2K + h] \cosh[-2K + h]}{\cosh^2[h]} \quad (2.14)$$

Now for the  $h'$  identity. Let's divide 3.12 by 3.13.

$$e^{2h'} = \frac{2e^h \cosh[2K + h]}{2e^{-h} \cosh[-2K + h]} \quad (2.15)$$

$$e^{2h'} = e^{2h} \frac{\cosh[2K + h]}{\cosh[-2K + h]} \quad (2.16)$$

Natural log both sides:

$$2h' = 2h + \ln \frac{\cosh[2K + h]}{\cosh[-2K + h]} \quad (2.17)$$

$$h' = h + \frac{1}{2} \ln \frac{\cosh[2K + h]}{\cosh[-2K + h]} \quad (2.18)$$

Oh wow hyperbolic cosine is even.

$$h' = h + \frac{1}{2} \ln \frac{\cosh[2K + h]}{\cosh[2K - h]} \quad (2.19)$$

For the last equation, let's multiply 3.12 by 3.13 and the square of 3.14.

$$A(K, h)^4 e^0 = (2e^h \cosh[2K + h])(2e^{-h} \cosh[-2K + h])(4 \cosh^2[h]) \quad (2.20)$$

$$A(K, h)^4 = 16 \cosh[2K + h] \cosh[-2K + h] \cosh^2[h] \quad (2.21)$$

Natural log both sides:

$$\ln A(K, h) = \frac{1}{4} \ln(16 \cosh[2K + h] \cosh[-2K + h] \cosh^2[h]) \quad (2.22)$$

This is what we want amen.

## Question 2.c

Show that the recursion relations have a line of trivial fixed points satisfying  $K^* = 0$  and arbitrary  $h^*$ , corresponding to the paramagnetic phase, and an unstable ferromagnetic fixed point at  $K^* = \infty, h^* = 0$ .

For  $K^* = 0(K = 0), h^*$ ,

$$K' = \frac{1}{4} \ln \frac{\cosh(h) \cosh(-h)}{\cosh^2(h)} = \frac{1}{4} \ln \frac{\cosh^2(h)}{\cosh^2(h)} = \frac{1}{4} \ln(1) = 0 \quad (2.23)$$

let's do  $h'$

$$h' = h^* = h + \frac{1}{2} \ln \left[ \frac{\cosh(h)}{\cosh(h)} \right] = h + \frac{1}{2} \ln[1] = h \quad (2.24)$$

Since this is linear, for  $K^* = 0$ , we have a line of trivial solutions.

### Question 2.d

Justify:

$$Z(K, h, N) = A(K, h)^{N/2} Z(K', h', N/2) \quad (2.25)$$

We have the familiar function for zero magnetic field.

$$Z(K, N) = A(K)^{N/2} Z(K', N/2) \quad (2.26)$$

Since we have it so that we have non-zero magnetic field, the extension is simply making  $A$  a function of  $h$  while also having the renormalized  $Z$ .

### Question 3

The partition function for the  $N$ -spin Ising chain can be written as the trace of the  $N$ th power of the transfer matrix  $\mathbf{T}$ . Another way to reduce the number of degrees of freedom is to describe the system in terms of two-spin cells. We write  $Z$  as:

$$Z = \text{Tr} \mathbf{T}^N = \text{Tr}(\mathbf{T}^2)^{N/2} = \text{Tr} \mathbf{T}'^{N/2} \quad (3.1)$$

The transfer matrix for two-spin cells,  $\mathbf{T}^2$ , can be written as

$$\mathbf{T}^2 = \mathbf{T} \mathbf{T} = \begin{pmatrix} e^{2K+2h} + e^{-2K} & e^h + e^{-h} \\ e^{-h} + e^h & e^{2K-2h} + e^{-2K} \end{pmatrix} \quad (3.2)$$

We require that  $\mathbf{T}'$  have the same form as  $\mathbf{T}$ :

$$\mathbf{T}' = C \begin{pmatrix} e^{K'+h'} & e^{-K'} \\ e^{-K'} & e^{K'-h'} \end{pmatrix} \quad (3.3)$$

A parameter  $C$  must be introduced because matching the two equations requires three matrix elements, which is impossible with only two variables  $K'$  and  $h'$ .

### Question 3.a

Show that the three unknowns satisfy the three conditions:

$$C e^{K'} e^{h'} = e^{2K+2h} + e^{-2K} \quad (3.4)$$

$$C e^{-K'} = e^h + e^{-h} \quad (3.5)$$

$$C e^{K'} e^{-h'} = e^{2K-2h} + e^{-2K} \quad (3.6)$$

The first condition is quite trivial. The top left element on  $\mathbf{T}'$  is (when absorbing the parameter)

$$C e^{K'+h'} \quad (3.7)$$

And through exponent rules this is:

$$Ce^{K'}e^{h'} \quad (3.8)$$

And since  $\mathbf{T}' = \mathbf{T}^2$

$$Ce^{K'}e^{h'} = e^{2K+2h} + e^{-2K} \quad (3.9)$$

The second condition is similar. Where we match the top right elements.

$$C(e^{-K'}) = Ce^{-K'} = e^h + e^{-h} \quad (3.10)$$

The third condition is then:

$$C(e^{K'}e^{-h'}) = Ce^{K'}e^{-h'} = Ce^{K'-h'} = e^{2K-2h} + e^{-2K} \quad (3.11)$$

### Question 3.b

Show that the solutions of the previous can be written as

$$e^{-2h'} = \frac{e^{2K-2h} + e^{-2K}}{e^{2K+2h} + e^{-2K}} \quad (3.12)$$

$$e^{4K'} = \frac{e^{4K} + e^{-2h} + e^{2h} + e^{-4K}}{(e^h + e^{-h})^2} \quad (3.13)$$

$$C^4 = [e^{4K} + e^{-2h} + e^{2h} + e^{-4K}][e^h + e^{-h}]^2 \quad (3.14)$$

For the first relation, let's divide equation 3.6 by 3.5.

$$\frac{Ce^{K'}e^{-h'}}{Ce^{K'}e^{h'}} = \frac{e^{-h'}}{e^{h'}} = e^{-2h'} \quad (3.15)$$

Using the RHS of those equations:

$$e^{-2h'} = \frac{e^{2K-2h} + e^{-2K}}{e^{2K+2h} + e^{-2K}} \quad (3.16)$$

The second relation can be shown through multiplying equations 3.4 and 3.6 and dividing by the square of 3.5

$$\frac{Ce^{K'}e^{h'}Ce^{K'}e^{-h'}}{C^2e^{-2K'}} = \frac{(e^{2K+2h} + e^{-2K})(e^{2K-2h} + e^{-2K})}{(e^h + e^{-h})^2} \quad (3.17)$$

Which then simplifies to:

$$\frac{C^2e^{h'-h'}}{C^2}e^{4K'} = \frac{e^{4K+0h} + e^{0K+2h} + e^{0K+2h} + e^{-4K}}{(e^h + e^{-h})^2} \quad (3.18)$$

Which then gives us:

$$e^{4K'} = \frac{e^{4K} + e^{-2h} + e^{2h} + e^{-4K}}{(e^h + e^{-h})^2} \quad (3.19)$$

The last relation can be shown by doing the same operation as the second relation, but multiply the square of 3.5 rather than divide.

$$Ce^{K'}e^{h'}Ce^{K'}e^{-h'}C^2e^{-2K'} = (e^{4K} + e^{-2h} + e^{2h} + e^{-4K})(e^h + e^{-h})^2 \quad (3.20)$$

Where we use results from the last derivation. This finally gives:

$$C^4 \frac{e^{2K'}}{e^{2K'}} \frac{e^{h'}}{e^{h'}} = C^4 = (e^{4K} + e^{-2h} + e^{2h} + e^{-4K})(e^h + e^{-h})^2 \quad (3.21)$$

Which is the final relation.

### Question 3.c

Show that the recursion relations in the previous reduce to

$$K' = R(K) = \frac{1}{2} \ln[\cosh(2K)] \quad (3.22)$$

for  $h = 0$ . For  $h \neq 0$  start from some initial state,  $K_0, h_0$  and calculate a typical renormalization group trajectory. To what phase (paramagnetic or ferromagnetic) does the fixed point correspond?

For  $h = 0$ , let's reduce 3.13.

$$e^{4K'} = \frac{e^{4K} + 1 + 1 + e^{-4K}}{(1 + 1)^2} \quad (3.23)$$

Critically we recognize that:

$$e^{4K} + 2 + e^{-4K} = (e^{2K} + e^{-2K})^2 \quad (3.24)$$

This gives:

$$e^{4K'} = \frac{(e^{2K} + e^{-2K})^2}{2^2} \quad (3.25)$$

Let's natural log both sides:

$$4K' = \ln \left[ \left[ \frac{(e^{2K} + e^{-2K})}{2} \right]^2 \right] \quad (3.26)$$

Simplify:

$$K' = \frac{1}{4} \ln[\cosh(2K)^2] = \frac{1}{2} \ln[\cosh(2K)] \quad (3.27)$$

For the  $h \neq 0$  case, we can use the relation for  $K'$  and  $h'$  from the results in question 2.

$$K' = \frac{1}{4} \ln \frac{\cosh(2K + h) \cosh(2K - h)}{\cosh^2 h} \quad (3.28)$$

$$h' = h + \frac{1}{2} \ln \left[ \frac{\cosh(2K + h)}{2K - h} \right] \quad (3.29)$$

Let's give  $K_0 = 0.5$  and  $h_0 = 0.5$ . I'll do a sample calculation and then do the rest with a computer.

$$K'(0.5, 0.5) = \frac{1}{4} \ln \frac{\cosh(2(0.5) + 0.5) \cosh(2(0.5) - 0.5)}{\cosh^2(0.5)} = \frac{1}{4} \ln \frac{(2.35...)(1.13...)}{1.27...} \quad (3.30)$$

$$K'(0.5, 0.5) = 0.184 \quad (3.31)$$



Now for  $h'$ :

$$h'(0.5, 0.5) = 0.5 + \frac{1}{2} \ln \left[ \frac{\cosh(2(0.5) + 0.5)}{2(0.5) - 0.5} \right] = 0.5 + \frac{1}{2} \ln \left[ \frac{(2.35...)}{0.5} \right] \quad (3.32)$$

$$h'(0.5, 0.5) = 1.27 \quad (3.33)$$

**Table 1:** Group trajectory calculation starting from initial state  $K_0, h_0$

Iteration	$K'$	$h'$
0	0.5	0.5
1	0.184	1.27
2	0.00942	undef

We see that  $K'$  tends to 0, while  $h'$  diverges to infinity. This corresponds to the paramagnetic phase. NOTE: I realized I copied down the equation for  $h'$  wrong, to save time I won't be redoing these calculations, but I believe the physics is the same.

## References